Fix FFI function definitions
Started trying to prove correctness properties for them and it turns
out that Aw8alloc doesn't work the way we thought it did. These new
definitions should be correct, though proving that still looks tough.
Some commented out attempts at the bottom.

botworld_serialiseScript.sml
@@ -375,19 +375,21 @@ val write_output_dec_def = Define`
 
 val length_rec_def = Define`
     length_rec bs n =
-      if EVERY (λb. b = 0w) bs
-      then INL (2 * n)
+      if EVERY (λb. b = 0w : word8) bs
+      then INL (2n * n)
       else INR (OPTION_BIND (parse_sexp (MAP (CHR o w2n) bs)) odestSXNUM)`;
+
+val get_input_length_loop_body_def = Define`
+ get_input_length_loop_body =
+           (Let (SOME "bs") (App Aw8alloc [Var(Short"n"); Lit(Word8 0w)])
+                (Let NONE (App (FFI 0) [Var(Short"bs")])
+                     (Mat (App Opapp [App Opapp [Var(Long "Botworld" "length_rec"); Var(Short"bs")]; Var(Short "n")])
+                          [(Pcon (SOME(Short "inl")) [Pvar "n"], App Opapp [Var(Short"f"); Var(Short"n")] )
+                          ;(Pcon (SOME(Short "inr")) [Pcon (SOME(Short "some")) [Pvar "len"]], Var(Short"len"))])))`
 
 val get_input_length_body_def = Define`
   get_input_length_body =
-    (Letrec [("f","n",
-                (Let (SOME "bs") (App Aw8alloc [Var(Short"n")])
-                (Let NONE (App (FFI 0) [Var(Short"bs")])
-                (Mat (App Opapp [App Opapp [Var(Long "Botworld" "length_rec"); Var(Short"bs")]; Var(Short "n")])
-                     [(Pcon (SOME(Short "inl")) [Pvar "n"], App Opapp [Var(Short"f"); Var(Short"n")] )
-                     ;(Pcon (SOME(Short "inr")) [Pcon (SOME(Short "some")) [Pvar "len"]], Var(Short"len"))
-                     ]))))] (App Opapp [Var(Short "f") ; Lit(IntLit 1)]))`;
+    (Letrec [("f","n",get_input_length_loop_body)] (App Opapp [Var(Short "f") ; Lit(IntLit 1)]))`;
 
 val get_input_length_dec_def = Define`
   get_input_length_dec = Dlet(Pvar "get_input_length") (Fun "x" get_input_length_body)`
@@ -395,12 +397,12 @@ val get_input_length_dec_def = Define`
 val get_output_length_body_def = Define`
   get_output_length_body =
   (Letrec [("f","n",
-                (Let (SOME "bs") (App Aw8alloc [Var(Short"n")])
-                (Let NONE (App (FFI 3) [Var(Short"bs")])
-                (Mat (App Opapp [App Opapp [Var(Long "Botworld" "length_rec"); Var(Short"bs")]; Var(Short "n")])
-                     [(Pcon (SOME(Short "inl")) [Pvar "n"], App Opapp [Var(Short"f"); Var(Short"n")] )
-                     ;(Pcon (SOME(Short "inr")) [Pcon (SOME(Short "some")) [Pvar "len"]], Var(Short"len"))
-                     ]))))] (App Opapp [Var(Short "f") ; Lit(IntLit 1)]))`;
+            (Let (SOME "bs") (App Aw8alloc [Var(Short"n"); Lit(Word8 0w)])
+                 (Let NONE (App (FFI 3) [Var(Short"bs")])
+                      (Mat (App Opapp [App Opapp [Var(Long "Botworld" "length_rec"); Var(Short"bs")]; Var(Short "n")])
+                           [(Pcon (SOME(Short "inl")) [Pvar "n"], App Opapp [Var(Short"f"); Var(Short"n")] )
+                           ;(Pcon (SOME(Short "inr")) [Pcon (SOME(Short "some")) [Pvar "len"]], Var(Short"len"))]))))] 
+          (App Opapp [Var(Short "f") ; Lit(IntLit 1)]))`;
 
 val get_output_length_dec_def = Define`
   get_output_length_dec = Dlet (Pvar "get_output_length") (Fun "x" get_output_length_body)`;
@@ -422,20 +424,49 @@ val read_output_dec_def = Define`
            (App Opapp [Var(Long "Botworld" "decode_output"); App Opapp [Var(Long "ByteArray" "toList") ; Var(Short"bs")]]))))`;
 
 (*
+val _ = register_type ``:'a + 'b``
+val _ = register_type ``:'a option``
+
+val _ = Globals.max_print_depth := 0;
+val evals = [evaluate_def, do_app_def, do_opapp_def, lookup_var_id_def, evalPropsTheory.build_rec_env_merge, 
+             evalPropsTheory.find_recfun_ALOOKUP, store_alloc_def, store_lookup_def, store_assign_def,
+             libTheory.opt_bind_def, rich_listTheory.EL_LENGTH_APPEND];
+val _ = Globals.max_print_depth := 10;
+
+val get_input_length_rec_thm = Q.store_thm("get_input_length_rec_thm",
+  `∀ m n s st env.
+   s.ffi.oracle = botworld_oracle ∧
+   s.ffi.ffi_state = st ∧
+   m = LENGTH (encode_observation st.bot_input) ∧
+   lookup_var_id (Short "n") env = SOME(Litv(IntLit &n)) ∧
+   lookup_var_id (Short "f") env = SOME(Recclosure env0 [("f","n",get_input_length_loop_body)] "f") ⇒
+   ∃ bs ck s'. 
+   evaluate s env [get_input_length_loop_body] = (s',Rval[Litv(IntLit (&m))]) ∧
+   s' = s with <| refs := MAP W8array bs ++ s.refs;
+                  clock := s.clock - ck |>`,
+   gen_tac \\ completeInduct_on `m` \\ rw[]
+   \\ rw[get_input_length_loop_body_def] \\ rw[evaluate_def, do_app_def] \\ rw evals
+)
 val get_input_length_thm = Q.store_thm("get_input_length_thm",
   `lookup_var_id (Long"Botworld""get_input_length") env = SOME (Closure env0 "x" get_input_length_body) ∧
    s.ffi.oracle = botworld_oracle ∧
-   evaluate s env [u] = (s,Rval[Conv NONE []]) ∧
+   evaluateg s env [u] = (s,Rval[Conv NONE []]) ∧
    evaluate s env [App Opapp [Var(Long"Botworld""get_input_length"); u]] = (s', res) ∧
+   Eval env (Var (Long "Botworld""length_rec")) ((LIST_TYPE WORD8 --> NUM --> SUM_TYPE NUM (OPTION_TYPE NUM)) length_rec) ∧
    res ≠ Rerr(Rabort Rtimeout_error)
    ⇒
    ∃ck bs.
-     s' = s with <| refs := W8array bs::s.refs;
+     s' = s with <| refs := MAP W8array bs ++ s.refs;
                     clock := s.clock - ck |>
      ∧ res = Rval[Litv(IntLit (&(LENGTH (encode_observation st.bot_input))))]`,
   rw[evaluate_def] \\ rfs[]
   \\ fs[do_opapp_def]
   \\ every_case_tac \\ fs[]
+  \\ qhdtm_x_assum `funBigStep$evaluate` mp_tac
+  \\ simp[get_input_length_body_def, evaluate_def, lookup_var_id_def, evalPropsTheory.build_rec_env_merge]
+  \\ simp[do_opapp_def, evalPropsTheory.find_recfun_ALOOKUP]
+  \\ rw[] \\ fs[] \\ pop_assum mp_tac
+  \\ simp[evalPropsTheory.build_rec_env_merge]
 *)
 
 val _ = export_theory()
